updates

Veritas.SeqAux.fst
@@ -185,7 +185,7 @@ let filter_index_map (#a:eqtype) (f:a -> bool) (s:seq a) (i:seq_index (filter f 
   Tot (j:seq_index s{index s j = index (filter f s) i}) =
   proj_index_map (filter f s) s (filter_is_proj_prf f s) i
 
-let rec filter_len_monotonic (#a:eqtype) (f:a -> bool) (s:seq a) (i:nat{i <= length s}):
+let rec lemma_filter_len_monotonic (#a:eqtype) (f:a -> bool) (s:seq a) (i:nat{i <= length s}):
   Lemma (requires (True))
         (ensures (length (filter f s) >= length (filter f (prefix s i))))
         (decreases (length s)) =
@@ -195,7 +195,7 @@ let rec filter_len_monotonic (#a:eqtype) (f:a -> bool) (s:seq a) (i:nat{i <= len
   else (
     let s' = prefix s (n - 1) in
     lemma_len_slice s 0 (n - 1);
-    filter_len_monotonic f s' i
+    lemma_filter_len_monotonic f s' i
   )
 
 let rank (#a:eqtype) (f:a -> bool)  (s:seq a) (i:nat{i <= length s})
@@ -209,7 +209,7 @@ let rank_increases_by_atmost_one (#a:eqtype) (f:a -> bool) (s:seq a)
 
 let filter_index_inv_map_aux (#a:eqtype) (f:a -> bool) (s:seq a) (i:seq_index s{f (index s i)}):
   Tot (seq_index (filter f s)) = 
-  filter_len_monotonic f s (i+1);
+  lemma_filter_len_monotonic f s (i+1);
   lemma_len_append (filter f (prefix s i)) (create 1 (index s i));
   rank f s i
 
@@ -244,111 +244,58 @@ let rec seq_refine_aux (#a:Type) (f:a -> bool) (s:seq a{forall (i:seq_index s). 
 let seq_refine (#a:Type) (f:a -> bool) (s:seq a{forall (i:seq_index s). f (index s i)}): Tot (seq (refine f))
   = seq_refine_aux f s
 
-let filter_index_map_monotonic (#a:eqtype) (f:a -> bool) (s:seq a) 
+let lemma_filter_index_map_monotonic (#a:eqtype) (f:a -> bool) (s:seq a) 
   (i:seq_index (filter f s))(j:seq_index (filter f s){j > i}):
   Lemma (filter_index_map f s i < filter_index_map f s j) = 
   lemma_proj_monotonic (filter f s) s (filter_is_proj_prf f s) i j
 
-
-(*
-
-
-
-
-
-
-
-
-
-let filter_index_map_aux (#a:eqtype) (f:a -> bool)  (s:seq a)
-  (i:seq_index s{f (index s i)}):
-  Tot (seq_index (filter f s)) =
-  filter_len_monotonic f s (i+1);
-  lemma_len_append (filter f (prefix s i)) (create 1 (index s i));
-  rank f s i
-
-let rec filter_index_map_correct (#a:eqtype) (f:a -> bool) (s:seq a) (i:seq_index s):
-  Lemma (requires (f (index s i)))
-        (ensures (index s i = index (filter f s) (filter_index_map_aux f s i)))
-        (decreases (length s)) =
-  let n = length s in
-  if n = 0 then ()
-  else if i = n - 1 then ()
-  else filter_index_map_correct f (prefix s (n - 1)) i
-
-let filter_index_map (#a:eqtype) (f:a -> bool) (s:seq a) (i:seq_index s{f (index s i)}):
-  Tot (j:seq_index (filter f s){index s i = index (filter f s) j}) =
-  filter_index_map_correct f s i;
-  filter_index_map_aux f s i
-
-let filter_index_map_monotonic (#a:eqtype) (f:a -> bool) (s:seq a)
-  (i:seq_index s) (j:seq_index s{j > i}):
-  Lemma (requires (f (index s i) && f (index s j)))
-        (ensures (filter_index_map f s i < filter_index_map f s j)) =
-  filter_len_monotonic f (prefix s j) (i + 1)
-
-
-let rec rank_search (#a:eqtype) (f:a -> bool) (s:seq a)
-                (r:seq_index (filter f s))
-                (i:nat{i <= length s && rank f s i > r})
-  : Tot (j:seq_index s{rank f s j = r && f (index s j)})
-    (decreases i) =
-  assert (i > 0);
-  if rank f s (i - 1) = r then (i - 1)
-  else (
-    rank_increases_by_atmost_one f s (i - 1);
-    rank_search f s r (i - 1)
-  )
-
-let filter_index_inv_map (#a:eqtype) (f:a -> bool)  (s:seq a) (i:seq_index (filter f s))
-  : Tot (j:seq_index s{f (index s j) && filter_index_map f s j = i}) =
-  rank_search f s i (length s)
-
-let filter_index_inv_map_monotonic (#a:eqtype) (f:a -> bool) (s: seq a)
-  (i:seq_index (filter f s)) (j: seq_index (filter f s) {j > i}):
-    Lemma (requires (True))
-          (ensures (filter_index_inv_map f s i < filter_index_inv_map f s j)) =
-  let i' = filter_index_inv_map f s i in
-  let j' = filter_index_inv_map f s j in
-  if i' < j' then () // nothing to prove
-  else if i' > j' then
-    filter_index_map_monotonic f s j' i'
-  else ()
+let lemma_filter_index_inv_map_monotonic (#a:eqtype) (f:a -> bool) (s: seq a)
+  (i:seq_index s) (j: seq_index s {j > i}):
+    Lemma (requires (f (index s i) /\ f (index s j)))
+          (ensures (filter_index_inv_map f s i < filter_index_inv_map f s j)) = 
+  lemma_filter_len_monotonic f (prefix s j) (i+1)
 
 let lemma_filter_maps_correct (#a:eqtype) (f:a -> bool) (s: seq a) (i:seq_index s):
   Lemma (requires (f (index s i)))
-        (ensures (filter_index_inv_map f s (filter_index_map f s i) = i)) =
-  let i' = filter_index_map f s i in
-  let i2 = filter_index_inv_map f s i' in
-  if i2 < i then
-    filter_index_map_monotonic f s i2 i
-  else if i2 > i then
-    filter_index_map_monotonic f s i i2
+        (ensures (filter_index_map f s (filter_index_inv_map f s i) = i)) = 
+  lemma_filter_maps_aux f s i
+
+let lemma_filter_maps_correct2 (#a:eqtype) (f:a -> bool) (s: seq a) (i: seq_index (filter f s)):
+  Lemma (filter_index_inv_map f s (filter_index_map f s i) = i) = 
+  let j = filter_index_map f s i in
+  let i' = filter_index_inv_map f s j in
+  let j' = filter_index_map f s i' in
+  lemma_filter_maps_correct f s j;
+  assert(j = j');  
+  if i < i' then
+    lemma_filter_index_map_monotonic f s i i'
+  else if i > i' then 
+    lemma_filter_index_map_monotonic f s i' i
   else ()
 
 let last_index_opt (#a:eqtype) (f:a -> bool) (s:seq a):
   Tot (option (i:seq_index s{f (index s i)})) =
   let fs = filter f s in
   if length fs = 0 then None
-  else Some (filter_index_inv_map f s ((length fs) - 1))
+  else Some (filter_index_map f s ((length fs) - 1))
 
 let lemma_last_index_correct1 (#a:eqtype) (f:a -> bool) (s:seq a) (i:seq_index s):
   Lemma (requires (exists_sat_elems f s /\ i > last_index f s))
         (ensures (not (f (index s i)))) =
   let j = last_index f s in
   if f (index s i) then
-    filter_index_map_monotonic f s j i
+    lemma_filter_index_inv_map_monotonic f s j i      
   else ()
 
 let lemma_last_index_correct2 (#a:eqtype) (f:a -> bool)  (s:seq a) (i:seq_index s):
   Lemma (requires (f (index s i)))
         (ensures (exists_sat_elems f s /\ last_index f s >= i)) =
   let n = length s in
-  let ri = filter_index_map f s i in
+  let ri = filter_index_inv_map f s i in
   assert (exists_sat_elems f s);
   let j = last_index f s in
-  if j < i then
-    filter_index_map_monotonic f s j i
+  if j < i then 
+    lemma_filter_index_inv_map_monotonic f s j i  
   else ()
 
 let lemma_last_index_prefix (#a:eqtype) (f:a -> bool) (s:seq a) (i:nat{i <= length s}):
@@ -360,7 +307,7 @@ let lemma_last_index_prefix (#a:eqtype) (f:a -> bool) (s:seq a) (i:nat{i <= leng
   lemma_prefix_index s i li;
   assert(f (index s' li));
   assert(li < length s');
-  let r' = filter_index_map f s' li in
+  let r' = filter_index_inv_map f s' li in
   assert(exists_sat_elems f s');
   let li' = last_index f s' in
   if li < li' then (
@@ -406,14 +353,14 @@ let lemma_last_index_last_elem_sat (#a:eqtype) (f:a -> bool) (s:seq a{length s >
 
 let first_index (#a:eqtype) (f:a -> bool) (s:seq a{exists_sat_elems f s})
   : Tot (i:seq_index s{f (index s i)}) =
-  filter_index_inv_map f s 0
+  filter_index_map f s 0
 
 let lemma_first_index_correct1 (#a:eqtype) (f:a -> bool) (s:seq a) (i:seq_index s):
   Lemma (requires (exists_sat_elems f s /\ i < first_index f s))
         (ensures (not (f (index s i)))) =
   let fi = first_index f s in
   if f (index s i) then
-    filter_index_map_monotonic f s i fi
+    lemma_filter_index_inv_map_monotonic f s i fi
   else ()
 
 let lemma_first_index_correct2 (#a:eqtype) (f:a -> bool) (s:seq a) (i:seq_index s):
@@ -456,4 +403,3 @@ let lemma_map_index (#a #b: Type) (f:a -> b) (s:seq a) (i:seq_index s):
   Lemma (requires (True))
         (ensures (f (index s i) == index (map f s) i)) =
   lemma_map_index_aux f s i
-*)
