Veritas.Interleave.fsti
@@ -1,0 +1,30 @@
+module Veritas.Interleave
+
+open FStar.Seq
+open Veritas.SeqAux
+
+(* interleaving of n sequences *)
+val interleave (#a:eqtype): seq a -> ss:(seq (seq a)) -> Type 
+
+(* if we have a proof of interleaving we can construct a mapping from 
+ * interleaved sequence to the sources *)
+val interleave_map (#a:eqtype) (s: seq a) (ss: seq (seq a)) 
+     (prf:interleave #a s ss) (i: seq_index s): 
+  Tot (j: (nat*nat){fst j < length ss /\
+                 snd j < length (index ss (fst j)) /\
+                 index (index ss (fst j)) (snd j) = index s i})
+
+(* inverse of interleave map *)
+val interleave_map_inv (#a:eqtype) (s: seq a) (ss: seq (seq a))
+      (prf:interleave #a s ss) (i: seq_index ss) (j: seq_index (index ss i)): 
+  Tot (k: seq_index s{index s k = index (index ss i) j})
+
+(* sortedness of a sequence *)
+type sorted (#a:Type) (lte: a -> a -> bool) (s: seq a) = 
+  forall (i:seq_index s). i > 0 ==> index s (i - 1) `lte` index s i
+
+(* sort-merge interleaving *)
+val sort_merge (#a:eqtype) (lte: a-> a-> bool) 
+               (ss: seq (seq a){forall (i:seq_index ss). sorted lte (index ss i)}): 
+  s:(seq a){interleave s ss /\ sorted lte s} 
+    
