Makefile
@@ -11,12 +11,12 @@ FLAKY=
 FSTAR_FILES := Veritas.BinTree.fsti Veritas.BinTree.fst \
                Veritas.Key.fsti Veritas.Record.fsti \
                Veritas.SeqAux.fsti Veritas.SeqAux.fst \
+               Veritas.State.fsti \
                Veritas.MultiSet.fsti Veritas.MultiSet.fst \
                Veritas.MultiSetHash.fsti Veritas.MultiSetHash.fst \
                Veritas.Hash.fsti \
-               Veritas.SeqOps.fsti Veritas.SeqOps.fst \
+               Veritas.Interleave.fsti \
                Veritas.Verifier.fst \
-               Veritas.State.fsti \
                Veritas.Verifier.Correctness.fst
 
 
